interface for Benton2004.DDCC

examples/rel/Benton2004.DDCC.fsti
@@ -14,74 +14,126 @@
    limitations under the License.
 *)
 module Benton2004.DDCC
+include Benton2004
 
-let holds_ns_f (#t: Type0) (x y: t): Lemma
+type per (t: Type0) = ( f: rel t { is_per f } )
+
+type nstype (t: Type0) = per t
+
+let ns_f (#t: Type0) : nstype t =
+  let f (x y: t) = False in
+  Classical.forall_intro_2 (holds_equiv f);
+  f
+
+val holds_ns_f (#t: Type0) (x y: t): Lemma
   (holds ns_f x y <==> False)
   [SMTPat (holds ns_f x y)]
-= holds_equiv ns_f x y
 
-let holds_ns_t (#t: Type0) (x y: t): Lemma
+let ns_t (#t: Type0) : nstype t =
+  let f (x y: t) = True in
+  Classical.forall_intro_2 (holds_equiv f);
+  f
+
+val holds_ns_t (#t: Type0) (x y: t): Lemma
   (holds ns_t x y <==> True)
   [SMTPat (holds ns_t x y)]
-= holds_equiv ns_t x y
 
-let holds_ns_singl (#t: Type0) (c: t) (x y: t) : Lemma
+let ns_singl (#t: Type0) (c: t) : nstype t =
+  let f (x y: t) = (x == c /\ y == c) in
+  Classical.forall_intro_2 (holds_equiv f);
+  f
+
+val holds_ns_singl (#t: Type0) (c: t) (x y: t) : Lemma
   (holds (ns_singl c) x y <==> (x == c /\ y == c))
   [SMTPat (holds (ns_singl c) x y)]
-= holds_equiv (ns_singl c) x y
 
-let holds_ns_delta (#t: Type0) (x y : t) : Lemma
+let ns_delta (#t: Type0) : nstype t =
+  let f (x y: t) = (x == y) in
+  Classical.forall_intro_2 (holds_equiv f);
+  f
+
+val holds_ns_delta (#t: Type0) (x y : t) : Lemma
   (holds ns_delta x y <==> x == y)
   [SMTPat (holds ns_delta x y)]
-= holds_equiv ns_delta x y
 
-let interpolable_ns_f #t : Lemma (interpolable #t ns_f) = ()
-let interpolable_ns_t #t : Lemma (interpolable #t ns_t) = ()
-let interpolable_ns_singl #t (c: t) : Lemma (interpolable (ns_singl c)) = ()
-let interpolable_ns_delta #t : Lemma (interpolable #t ns_delta) = ()
+val interpolable_ns_f (#t:Type) : Lemma (interpolable #t ns_f)
+val interpolable_ns_t (#t:Type) : Lemma (interpolable #t ns_t)
+val interpolable_ns_singl (#t:Type) (c: t) : Lemma (interpolable (ns_singl c))
+val interpolable_ns_delta (#t:Type) : Lemma (interpolable #t ns_delta)
 
-#set-options "--z3rlimit 128 --max_fuel 8 --max_ifuel 8"
+type sttype = (f: per heap { interpolable f } )
 
-let holds_st_nil
+let st_nil: sttype =
+  let f (x y : heap) : GTot Type0 = True in
+  f
+
+val holds_st_nil
   (x y: heap)
 : Lemma
   (holds st_nil x y <==> True)
   [SMTPat (holds st_nil x y)]
-= Classical.forall_intro_2 (holds_equiv st_nil)
 
-let holds_st_var
+let st_var
+  (x: var)
+  (v: nstype int)
+: GTot sttype
+= let f (s1 s2: heap) : GTot Type0 = holds v (sel s1 x) (sel s2 x) in
+  Classical.forall_intro_2 (holds_equiv f);
+  f
+
+val holds_st_var
   (x: var)
   (v: nstype int)
   (a b: heap)
 : Lemma
   (holds (st_var x v) a b <==> holds v (sel a x) (sel b x))
   [SMTPat (holds (st_var x v) a b)]
-= holds_equiv (st_var x v) a b
 
-let holds_st_intersect
+let st_intersect
+  (p1 p2: sttype)
+: GTot sttype
+= intersect p1 p2
+
+val holds_st_intersect
   (ns1 ns2: sttype)
   (x y: heap)
 : Lemma
   (holds (st_intersect ns1 ns2) x y <==> (holds ns1 x y /\ holds ns2 x y))
   [SMTPat (holds (st_intersect ns1 ns2) x y)]
-= ()
 
-let st_fresh_in_nil
+let st_fresh_in
+  (x: var)
+  (p: sttype)
+: GTot Type0
+= forall s1 s1' s2 s2' . 
+  (holds p s1 s2 /\ (
+    forall y . y <> x ==> (sel s1' y == sel s1 y /\ sel s2' y == sel s2 y)
+  )) ==>
+  holds p s1' s2'
+
+val st_fresh_in_nil
   (x: var)
 : Lemma
   (x `st_fresh_in` st_nil)
-= ()
 
-let st_fresh_in_var
+let st_cons
+  (p: sttype)
+  (x: var)
+  (v: nstype int)
+: Ghost sttype
+  (requires (x `st_fresh_in` p))
+  (ensures (fun _ -> True))
+= st_intersect p (st_var x v)
+
+val st_fresh_in_var
   (x: var)
   (v: nstype int)
   (y: var)
 : Lemma
   (requires (y <> x))
   (ensures (y `st_fresh_in` (st_var x v)))
-= ()
 
-let st_fresh_in_intersect
+val st_fresh_in_intersect
   (x: var)
   (p1 p2: sttype)
 : Lemma
@@ -90,9 +142,8 @@ let st_fresh_in_intersect
     x `st_fresh_in` p2
   ))
   (ensures (x `st_fresh_in` (st_intersect p1 p2)))
-= ()
 
-let st_fresh_in_cons
+val st_fresh_in_cons
   (p: sttype)
   (x: var)
   (v: nstype int)
@@ -107,35 +158,28 @@ let st_fresh_in_cons
     x `st_fresh_in` p /\
     y `st_fresh_in` (st_cons p x v)
   ))
-= ()
 
-let subtype_ns_f (#t: Type0) (phi: nstype t) : Lemma
+val subtype_ns_f (#t: Type0) (phi: nstype t) : Lemma
   (included ns_f phi)
-= ()
 
-let subtype_ns_singl_delta (#t: Type0) (c: t) : Lemma
+val subtype_ns_singl_delta (#t: Type0) (c: t) : Lemma
   (ns_singl c `included` ns_delta)
-= ()
 
-let subtype_ns_t (#t: Type0) (phi: nstype t) : Lemma
+val subtype_ns_t (#t: Type0) (phi: nstype t) : Lemma
   (included phi ns_t)
-= ()
 
-let subtype_st_nil (phi: sttype) : Lemma
+val subtype_st_nil (phi: sttype) : Lemma
   (included phi st_nil)
-= ()
 
-let subtype_st_f (phi phi' : sttype) (x: var) : Lemma
+val subtype_st_f (phi phi' : sttype) (x: var) : Lemma
   (requires (x `st_fresh_in` phi))
   (ensures (x `st_fresh_in` phi /\ included (st_cons phi x ns_f) phi'))
-= ()
 
-let subtype_st_t (phi phi' : sttype) (x: var) : Lemma
+val subtype_st_t (phi phi' : sttype) (x: var) : Lemma
   (requires (x `st_fresh_in` phi' /\ included phi phi'))
   (ensures (x `st_fresh_in` phi' /\ included phi (st_cons phi' x ns_t)))
-= ()
 
-let subtype_st_cons (phi phi' : sttype) (f f' : nstype int) (x: var) : Lemma
+val subtype_st_cons (phi phi' : sttype) (f f' : nstype int) (x: var) : Lemma
   (requires (
     included phi phi' /\
     included f f' /\
@@ -147,17 +191,15 @@ let subtype_st_cons (phi phi' : sttype) (f f' : nstype int) (x: var) : Lemma
     x `st_fresh_in` phi' /\
     included (st_cons phi x f) (st_cons phi' x f')
   ))
-= ()
 
-let eval_equiv_reified
+val eval_equiv_reified
   (#t: Type0)
   (p: sttype)
   (e: nstype t)
   (f f': reified_exp t)
 : GTot Type0
-= Benton2004.eval_equiv_reified p e f f'
 
-let eval_equiv_reified_elim
+val eval_equiv_reified_elim
   (#t: Type0)
   (p: sttype)
   (e: nstype t)
@@ -166,38 +208,33 @@ let eval_equiv_reified_elim
 : Lemma
   (requires (eval_equiv_reified p e f f' /\ holds p s s'))
   (ensures (holds e (fst (f s)) (fst (f' s'))))
-= ()  
 
-let terminates_equiv_reified
+val terminates_equiv_reified
   (p : sttype)
   (f f' : reified_computation)
 : GTot Type0
-= Benton2004.terminates_equiv_reified p f f'
 
-let terminates_equiv_reified_elim
+val terminates_equiv_reified_elim
   (p : sttype)
   (f f' : reified_computation)
   (s s' : heap)
 : Lemma
   (requires (terminates_equiv_reified p f f' /\ holds p s s'))
   (ensures (terminates_on f s <==> terminates_on f' s'))
-= ()
 
-let exec_equiv_reified
+val exec_equiv_reified
   (p p' : sttype)
   (f f' : reified_computation)
 : GTot Type0
-= Benton2004.exec_equiv_reified p p' f f'
 
-let exec_equiv_reified_terminates
+val exec_equiv_reified_terminates
   (p p' : sttype)
   (f f' : reified_computation)
 : Lemma
   (requires (exec_equiv_reified p p' f f'))
   (ensures (terminates_equiv_reified p f f'))
-= ()
 
-let exec_equiv_reified_elim
+val exec_equiv_reified_elim
   (p p' : sttype)
   (f f' : reified_computation)
   (s s' : heap)
@@ -205,9 +242,16 @@ let exec_equiv_reified_elim
 : Lemma
   (requires (exec_equiv_reified p p' f f' /\ holds p s s' /\ fst (f fuel s) == true /\ fst (f' fuel s') == true))
   (ensures (holds p' (snd (f fuel s)) (snd (f' fuel s'))))
-= ()
 
-let eval_equiv_sym
+let exec_equiv
+  (p p' : sttype)
+  (f f' : computation)
+: GTot Type0
+= let f = reify_computation f in
+  let f' = reify_computation f' in
+  exec_equiv_reified p p' f f'
+
+val eval_equiv_sym
   (#t: Type0)
   (p: sttype)
   (e: nstype t)
@@ -215,17 +259,15 @@ let eval_equiv_sym
 : Lemma
   (requires (eval_equiv p e f f'))
   (ensures (eval_equiv p e f' f))
-= Benton2004.eval_equiv_sym p e f f'
 
-let exec_equiv_sym
+val exec_equiv_sym
   (p p': sttype)
   (f f' : computation)
 : Lemma
   (exec_equiv p p' f f' <==> exec_equiv p p' f' f)
   [SMTPat (exec_equiv p p' f f')]
-= Benton2004.exec_equiv_sym p p' f f'
 
-let eval_equiv_trans
+val eval_equiv_trans
   (#t: Type0)
   (p: sttype)
   (e: nstype t)
@@ -233,17 +275,15 @@ let eval_equiv_trans
 : Lemma
   (requires (eval_equiv p e f1 f2 /\ eval_equiv p e f2 f3))
   (ensures (eval_equiv p e f1 f3))
-= Benton2004.eval_equiv_trans p e f1 f2 f3
 
-let exec_equiv_reified_trans
+val exec_equiv_reified_trans
   (p p': sttype)
   (f1 f2 f3 : reified_computation)
 : Lemma
   (requires (exec_equiv_reified p p' f1 f2 /\ exec_equiv_reified p p' f2 f3))
   (ensures (exec_equiv_reified p p' f1 f3))
-= Benton2004.exec_equiv_reified_trans p p' f1 f2 f3
 
-let exec_equiv_trans
+val exec_equiv_trans
   (p p' : sttype)
   (c1 c2 c3 : computation)
 : Lemma
@@ -257,10 +297,6 @@ let exec_equiv_trans
     [SMTPat (exec_equiv p p' c1 c2); SMTPat (exec_equiv p p' c1 c3)];
     [SMTPat (exec_equiv p p' c2 c3); SMTPat (exec_equiv p p' c1 c3)];
   ]]
-= let z1 = reify_computation c1 in
-  let z2 = reify_computation c2 in
-  let z3 = reify_computation c3 in
-  exec_equiv_reified_trans p p' z1 z2 z3
 
 (* Subtyping and structural *)
 
@@ -276,7 +312,7 @@ let d_ct1
 >>
 *)
 
-let d_ct
+val d_ct
   (c c' : computation)
   (p p' : sttype)
   (x: var)
@@ -284,18 +320,16 @@ let d_ct
   (requires (x `st_fresh_in` p))
   (ensures (x `st_fresh_in` p /\ exec_equiv (st_cons p x ns_f) p' c c'))
   [SMTPat (exec_equiv (st_cons p x ns_f) p' c c')]
-= ()
 
-let d_et1
+val d_et1
   (#t: Type0)
   (f f' : exp t)
   (p: sttype)
 : Lemma
   (eval_equiv p ns_t f f')
   [SMTPat (eval_equiv p ns_t f f')]
-= ()
 
-let d_et2
+val d_et2
   (#t: Type0)
   (f f' : exp t)
   (p: sttype)
@@ -305,9 +339,16 @@ let d_et2
   (requires (x `st_fresh_in` p))
   (ensures (x `st_fresh_in` p /\ eval_equiv (st_cons p x ns_f) p' f f'))
   [SMTPat (eval_equiv (st_cons p x ns_f) p' f f')]
-= ()
 
-let d_esub
+let d_esym = eval_equiv_sym
+
+let d_etr = eval_equiv_trans
+
+let d_csym = exec_equiv_sym
+
+let d_ctr = exec_equiv_trans
+
+val d_esub
   (#t: Type0)
   (f f' : exp t)
   (ph ph': sttype)
@@ -320,9 +361,8 @@ let d_esub
   ))
   (ensures (eval_equiv ph' p' f f'))
   [SMTPat (eval_equiv ph' p' f f'); SMTPat (eval_equiv ph p f f')]
-= Benton2004.d_esub f f' ph ph' p p'
 
-let d_csub
+val d_csub
   (p1 p2 p1' p2' : sttype)
   (f f' : computation)
 : Lemma
@@ -333,11 +373,10 @@ let d_csub
   ))
   (ensures (exec_equiv p1' p2' f f'))
   [SMTPat (exec_equiv p1' p2' f f'); SMTPat (exec_equiv p1 p2 f f')]
-= Benton2004.d_csub p1 p2 p1' p2' f f'
 
 (* Expressions *)
 
-let d_v
+val d_v
   (x: var)
   (p: sttype)
   (f: nstype int)
@@ -345,18 +384,19 @@ let d_v
   (requires (x `st_fresh_in` p))
   (ensures (x `st_fresh_in` p /\ eval_equiv (st_cons p x f) f (evar x) (evar x)))
   [SMTPat (eval_equiv (st_cons p x f) f (evar x) (evar x))]
-= ()
 
-let eval_equiv_const
+val eval_equiv_const
   (#t: Type0)
   (c: t)
   (p: sttype)
 : Lemma
   (eval_equiv p (ns_singl c) (const c) (const c))
   [SMTPat (eval_equiv p (ns_singl c) (const c) (const c))]
-= ()
 
-let d_op
+let d_n = eval_equiv_const #int
+let d_b = eval_equiv_const #bool
+
+val d_op
   (#from #to: Type0)
   (op: (from -> from -> Tot to))
   (e1 e1' e2 e2': exp from)
@@ -370,18 +410,16 @@ let d_op
     op_abs op ns1 ns2 ns
   ))
   (ensures (eval_equiv phi ns (eop op e1 e2) (eop op e1' e2')))
-= Benton2004.d_op op e1 e1' e2 e2' ns1 ns2 ns phi
 
 (* Commands *)
 
-let d_skip
+val d_skip
   (p: sttype)
 : Lemma
   (exec_equiv p p skip skip)
   [SMTPat (exec_equiv p p skip skip)]
-= Benton2004.d_skip p
 
-let d_assign
+val d_assign
   (p: sttype)
   (x: var)
   (f f': nstype int)
@@ -396,9 +434,8 @@ let d_assign
     exec_equiv (st_cons p x f) (st_cons p x f') (assign x e) (assign x e')
   ))
   [SMTPat (exec_equiv (st_cons p x f) (st_cons p x f') (assign x e) (assign x e'))]  
-= ()
 
-let d_seq
+val d_seq
   (p0 p1 p2 : sttype)
   (c01 c01' c12 c12' : computation)
 : Lemma
@@ -414,11 +451,8 @@ let d_seq
     [SMTPat (exec_equiv p0 p2 (seq c01 c12) (seq c01' c12')); SMTPat (exec_equiv p1 p2 c12 c12')];
     [SMTPat (exec_equiv p0 p1 c01 c01'); SMTPat (exec_equiv p1 p2 c12 c12')];
   ]]
-= Benton2004.d_seq p0 p1 p2 c01 c01' c12 c12'
 
-#set-options "--z3rlimit 1024"
-
-let d_ifthenelse
+val d_ifthenelse
   (b b' : exp bool)
   (c1 c1' c2 c2' : computation)
   (phi phi' : sttype)
@@ -430,9 +464,8 @@ let d_ifthenelse
   ))
   (ensures (exec_equiv phi phi' (ifthenelse b c1 c2) (ifthenelse b' c1' c2')))
   [SMTPat (exec_equiv phi phi' (ifthenelse b c1 c2) (ifthenelse b' c1' c2'))]
-= ()
 
-let rec d_whl_terminates
+val d_whl_terminates
   (b b' : exp bool)
   (c c' : computation)
   (phi : sttype)
@@ -449,45 +482,8 @@ let rec d_whl_terminates
     terminates_on (reify_computation (while b' c')) s0'
   ))
   (decreases fuel)
-= let fc = reify_computation c in
-  let fc' = reify_computation c' in
-  let f = reify_computation (while b c) in
-  let f' = reify_computation (while b' c') in
-  let e = fst (reify_exp b s0) in
-  assert (e == fst (reify_exp b' s0'));
-  if e
-  then begin
-    assert (terminates_on fc' s0');
-    let g
-      (fuel0: nat)
-    : Lemma
-      (requires (fst (fc' fuel0 s0') == true))
-      (ensures (terminates_on f' s0'))
-    = let fuel1 = fuel + fuel0 in
-      assert (fc' fuel1 s0' == fc' fuel0 s0');
-      assert  (fc fuel1 s0 == fc fuel s0);
-      let s1 = snd (fc fuel1 s0) in
-      let s1' = snd (fc' fuel1 s0') in
-      assert (holds phi s1 s1');
-      assert (f fuel s0 == f (fuel - 1) s1);
-      assert (f' fuel1 s0' == f' (fuel1 - 1) s1');
-      d_whl_terminates b b' c c' phi s1 s1' (fuel - 1);
-      let g'
-        (fuel2 : nat)
-      : Lemma
-        (requires (fst (f' fuel2 s1') == true))
-        (ensures (terminates_on f' s0'))
-      = let fuel3 = fuel1 + fuel2 + 1 in
-        assert (fc' fuel3 s0' == fc' fuel1 s0');
-        assert (f' fuel3 s0' == f' (fuel3 - 1) s1')
-      in
-      Classical.forall_intro (Classical.move_requires g')
-    in
-    Classical.forall_intro (Classical.move_requires g)
-  end else
-    assert (f' fuel s0' == (true, s0'))
 
-let d_whl
+val d_whl
   (b b' : exp bool)
   (c c' : computation)
   (phi : sttype)
@@ -498,75 +494,18 @@ let d_whl
   ))
   (ensures (exec_equiv phi phi (while b c) (while b' c')))
   [SMTPat (exec_equiv phi phi (while b c) (while b' c'))]
-= let eb = reify_exp b in
-  let eb' = reify_exp b' in
-  let eb_rel : squash (eval_equiv_reified phi ns_delta eb eb') = () in
-  let fc = reify_computation c in
-  let fc' = reify_computation c' in
-  let c_rel : squash (exec_equiv_reified phi phi fc fc') = () in
-  let f = reify_computation (while b c) in
-  let f' = reify_computation (while b' c') in
-  let prf1
-    (s0 s0' : heap)
-  : Lemma
-    (requires (holds phi s0 s0'))
-    (ensures (terminates_on f s0 <==> terminates_on f' s0'))
-  = exec_equiv_sym phi phi c c' ;
-    eval_equiv_sym phi ns_delta b b' ;
-    Classical.forall_intro (Classical.move_requires (d_whl_terminates b b' c c' phi s0 s0'));
-    Classical.forall_intro (Classical.move_requires (d_whl_terminates b' b c' c phi s0' s0))
-  in
-  Classical.forall_intro_2 (fun x -> Classical.move_requires (prf1 x));
-  let rec prf2
-    (fuel: nat)
-    (s0 s0' : heap)
-  : Lemma
-    (requires (
-      holds phi s0 s0' /\
-      fst (f fuel s0) == true /\
-      fst (f' fuel s0') == true
-    ))
-    (ensures (
-      holds phi (snd (f fuel s0)) (snd (f' fuel s0'))
-    ))
-    (decreases fuel)
-  = let e = fst (eb s0) in
-    let e' = fst (eb' s0') in
-    assert (holds phi s0 s0');
-    let e_rel : squash (holds ns_delta e e') =
-      eb_rel;
-      ()
-    in
-    assert (e == fst (eb' s0'));
-    if e
-    then begin
-      let k = fc fuel s0 in
-      let k' = fc' fuel s0' in
-      let s1 = snd k in
-      let s1' = snd k' in
-      let s_rel : squash (holds phi s1 s1') =
-        c_rel;
-        ()
-      in
-      assert (f fuel s0 == f (fuel - 1) s1);
-      assert (f' fuel s0' == f' (fuel - 1) s1');
-      prf2 (fuel - 1) s1 s1'
-    end else ()
-  in
-  Classical.forall_intro_3 (fun x y -> Classical.move_requires (prf2 x y))
 
 (* 3.1 Basic equations *)
 
-let d_su1
+val d_su1
   (c: computation)
   (phi phi' : sttype)
 : Lemma
   (requires (exec_equiv phi phi' c c))
   (ensures (exec_equiv phi phi' (seq skip c) c))
   [SMTPat (exec_equiv phi phi' (seq skip c) c)]
-= Benton2004.d_su1 c phi phi'
 
-let d_su1'
+val d_su1'
   (c c' c'' : computation)
   (phi phi' phi'' : sttype)
 : Lemma
@@ -580,9 +519,8 @@ let d_su1'
     [SMTPat (exec_equiv phi phi'' (seq c c') c''); SMTPat (exec_equiv phi' phi'' c' c'')];
     [SMTPat (exec_equiv phi phi' c skip); SMTPat (exec_equiv phi' phi'' c' c'')];
   ]]
-= Benton2004.d_su1' c c' c'' phi phi' phi''
 
-let d_su1''
+val d_su1''
   (c c' c'' : computation)
   (phi phi' phi_ phi'' : sttype)
 : Lemma
@@ -593,27 +531,24 @@ let d_su1''
   ))
   (ensures (exec_equiv phi phi'' (seq c c') c''))
   [SMTPat (exec_equiv phi phi' c skip); SMTPat (exec_equiv phi_ phi'' c' c'')]
-= d_su1' c c' c'' phi phi_ phi''
 
-let d_su2
+val d_su2
   (c: computation)
   (phi phi' : sttype)
 : Lemma
   (requires (exec_equiv phi phi' c c))
   (ensures (exec_equiv phi phi' (seq c skip) c))
   [SMTPat (exec_equiv phi phi' (seq c skip) c)]
-= Benton2004.d_su2 c phi phi'
 
-let d_assoc
+val d_assoc
   (c1 c2 c3: computation)
   (phi phi' : sttype)
 : Lemma
   (requires (exec_equiv phi phi' (seq (seq c1 c2) c3) (seq (seq c1 c2) c3)))
   (ensures (exec_equiv phi phi' (seq (seq c1 c2) c3) (seq c1 (seq c2 c3))))
   [SMTPat (exec_equiv phi phi' (seq (seq c1 c2) c3) (seq c1 (seq c2 c3)))]
-= Benton2004.d_assoc c1 c2 c3 phi phi'
 
-let d_cc
+val d_cc
   (b: exp bool)
   (c1 c2 c3: computation)
   (phi phi' phi'' : sttype)
@@ -630,27 +565,24 @@ let d_cc
     [SMTPat (exec_equiv phi phi'' (seq (ifthenelse b c1 c2) c3) (ifthenelse b (seq c1 c3) (seq c2 c3))); SMTPat (exec_equiv phi' phi'' c3 c3)];
     [SMTPat (exec_equiv phi phi' (ifthenelse b c1 c2) (ifthenelse b c1 c2)); SMTPat (exec_equiv phi' phi'' c3 c3)];
   ]]
-= Benton2004.d_cc b c1 c2 c3 phi phi' phi''
 
-let d_lu1
+val d_lu1
   (b: exp bool)
   (c: computation)
   (phi phi' : sttype)
 : Lemma
   (requires (exec_equiv phi phi' (while b c) (while b c)))
   (ensures (exec_equiv phi phi' (while b c) (ifthenelse b (seq c (while b c)) skip)))
-= Benton2004.d_lu1 b c phi phi'
 
-let d_lu2
+val d_lu2
   (b: exp bool)
   (c: computation)
   (phi phi' : sttype)
 : Lemma
   (requires (exec_equiv phi phi' (while b c) (while b c)))
   (ensures (exec_equiv phi phi' (while b c) (while b (seq c (ifthenelse b c skip)))))
-= Benton2004.d_lu2 b c phi phi'
 
-let d_sas
+val d_sas
   (x: var)
   (phi: sttype)
   (f: nstype int)
@@ -663,13 +595,12 @@ let d_sas
     exec_equiv (st_cons phi x f) (st_cons phi x f) (assign x (evar x)) skip
   ))
   [SMTPat (exec_equiv (st_cons phi x f) (st_cons phi x f) (assign x (evar x)) skip)]
-= ()
 
 (* 3.2 Optimizing Transformations *)
 
 (* Dead assignment elimination *)
 
-let d_das
+val d_das
   (x: var)
   (e: exp int)
   (phi: sttype)
@@ -681,11 +612,10 @@ let d_das
     exec_equiv (st_cons phi x f) (st_cons phi x ns_t) (assign x e) skip
   ))
   [SMTPat (exec_equiv (st_cons phi x f) (st_cons phi x ns_t) (assign x e) skip)]
-= assert (Benton2004.mention (reify_exp e)) // TODO: WHY is this necessary?
 
 (* Equivalent branches for conditional *)
 
-let d_bre
+val d_bre
   (c1 c2 c0: computation)
   (phi phi' : sttype)
   (b: exp bool)
@@ -696,11 +626,10 @@ let d_bre
   ))
   (ensures (exec_equiv phi phi' (ifthenelse b c1 c2) c0))
   [SMTPat (exec_equiv phi phi' (ifthenelse b c1 c2) c0)]
-= Benton2004.d_bre c1 c2 c0 phi phi' b
 
 (* Constant folding *)
 
-let d_cf
+val d_cf
   (t: Type0)
   (f: exp t)
   (c: t)
@@ -709,11 +638,10 @@ let d_cf
   (requires (eval_equiv phi (ns_singl c) f f))
   (ensures (eval_equiv phi (ns_singl c) f (const c)))
   [SMTPat (eval_equiv phi (ns_singl c) f (const c))]
-= ()
 
 (* Known branch *)
 
-let d_kb
+val d_kb
   (v: bool)
   (b: exp bool)
   (phi: sttype)
@@ -726,11 +654,13 @@ let d_kb
   ))
   (ensures (exec_equiv phi phi' (ifthenelse b c1 c2) c'))
   [SMTPat (eval_equiv phi (ns_singl v) b b); SMTPat (exec_equiv phi phi' (ifthenelse b c1 c2) c')]
-= ()
+
+let d_kbt = d_kb true
+let d_kbf = d_kb false
 
 (* Dead while *)
 
-let d_dwh
+val d_dwh
   (b: exp bool)
   (phi: sttype)
   (c: computation)
@@ -738,11 +668,10 @@ let d_dwh
   (requires (eval_equiv phi (ns_singl false) b b))
   (ensures (exec_equiv phi phi (while b c) skip))
   [SMTPat (exec_equiv phi phi (while b c) skip)]
-= ()
 
 (* Divergence *)
 
-let d_div
+val d_div
   (b: exp bool)
   (c: computation)
   (phi phi' : sttype)
@@ -754,48 +683,3 @@ let d_div
   (ensures (
     exec_equiv phi phi' (while b c) (while b c)
   ))
-= let f = reify_computation (while b c) in
-  let e = reify_exp b in
-  let e_rel : squash (eval_equiv phi (ns_singl true) b b) = () in
-  let fc = reify_computation c in
-  let f_rel : squash (exec_equiv_reified phi phi fc fc) = () in
-  let rec prf
-    (s0 s0' : heap)
-    (fuel: nat)
-  : Lemma
-    (requires (holds phi s0 s0'))
-    (ensures (fst (f fuel s0) == false))
-    (decreases fuel)
-  = let _ : squash (e s0 == (true, s0) /\ e s0' == (true, s0')) =
-      e_rel;
-      ()
-    in
-    let k = fc fuel s0 in
-    if fst k
-    then
-      let s1 = snd k in
-      if fuel = 0
-      then assert (fst (f fuel s0) == false)
-      else begin
-        assert (terminates_on fc s0);
-        assert (terminates_on fc s0');
-        let g
-          (fuel' : nat)
-        : Lemma
-          (requires (fst (fc fuel' s0') == true))
-          (ensures (fst (f fuel s0) == false))
-        = let s1' = snd (fc fuel' s0') in
-          assert (fc (fuel + fuel') s0 == fc fuel s0);
-          assert (fc (fuel + fuel') s0' == fc fuel' s0');
-          assert (f fuel s0 == f (fuel - 1) s1);
-          let _ : squash (holds phi s1 s1') =
-            f_rel;
-            ()
-          in
-          prf s1 s1' (fuel - 1)
-        in
-        Classical.forall_intro (Classical.move_requires g)
-    end else
-      assert (fst (f fuel s0) == false)
-  in
-  Classical.forall_intro_3 (fun x y -> Classical.move_requires (prf x y))
